bedrock2/src/bedrock2/SepCalls.v
@@ -1,0 +1,224 @@
+(* Separation logic automation for a general notion of function call,
+   based on "call lemmas" of the form
+
+   seps [...] mOld /\ (forall mNew vals, callPost vals -> seps [...] mNew -> finalPost) ->
+   executing a snippet of code satisfies finalPost
+
+   Applying the call lemma is not handled by this file, but solving the above conjunction
+   (except for solving finalPost) is. *)
+
+Require Export Coq.ZArith.ZArith. Open Scope Z_scope.
+Require Import coqutil.Z.Lia.
+Require Export coqutil.Byte.
+Require Import coqutil.Datatypes.HList.
+Require Import coqutil.Datatypes.PropSet.
+Require Export coqutil.Datatypes.Inhabited.
+Require Import coqutil.Tactics.rewr coqutil.Tactics.rdelta.
+Require Import Coq.Program.Tactics.
+Require Export coqutil.Tactics.Tactics.
+Require Export coqutil.Tactics.autoforward.
+Require Export coqutil.Map.Interface coqutil.Map.Properties coqutil.Map.OfListWord.
+Require Export coqutil.Word.Interface coqutil.Word.Properties.
+Require Import coqutil.Sorting.OrderToPermutation.
+Require Export coqutil.Tactics.fwd.
+Require Import coqutil.Tactics.ltac_list_ops.
+Require Export bedrock2.Lift1Prop.
+Require Export bedrock2.Map.Separation bedrock2.Map.SeparationLogic.
+Require Import bedrock2.Array.
+Require Export bedrock2.ZnWords.
+Require Import bedrock2.ptsto_bytes bedrock2.Scalars.
+Require Import bedrock2.groundcbv.
+Require Export bedrock2.TacticError.
+Require Import Coq.Strings.String. Open Scope string_scope.
+Export List.ListNotations. Open Scope list_scope.
+
+Section SepLog.
+  Context {width: Z} {word: word.word width} {mem: map.map word byte}.
+  Context {word_ok: word.ok word} {mem_ok: map.ok mem}.
+
+  (* Hides a sep behind a definition so that flattening operations keep
+     memPred and its associated purePred together as one clause *)
+  Definition with_pure(memPred: mem -> Prop)(purePred: Prop): mem -> Prop :=
+    sep memPred (emp purePred).
+
+  (* R, typically instantiated to `seps [whatever; is; left]`, appears twice:
+     On the left of the impl1 (this determines its value), and as the first
+     element of the `seps` on the right (there, it is an evar for the frame).
+     P is the continuation postcondition. *)
+  Lemma impl1_done: forall (R: mem -> Prop) (P: Prop),
+      P -> impl1 R (seps [R; emp P]).
+  Proof.
+    unfold impl1, seps. intros. apply sep_emp_r. auto.
+  Qed.
+
+  (* All arguments except stmt are just ghost parameters to guide typeclass search.
+     The shape of stmt will typically be
+       forall valAll valPart valFrame1 ... valFrameN,
+         sidecondition saying that assembling valPart valFrame1 ... valFrameN = valAll ->
+         iff1 (seps [addrPart |-> predPart valPart; Frame...]) (addrAll |-> predAll valAll)
+     but since that's a variable number of universally quantified variables, it would
+     be a bit cumbersome to enforce that shape, and since it's not needed to enforce it,
+     we don't.
+     Note that stmt needs to be not only applicable to split oldAll into oldPart and a
+     frame, but also to merge back a newPart and newFrame (potentially modified as well,
+     eg if a function separately takes two record fields) into a newAll.
+     So stmt needs to be more general than oldAll/oldPart.
+     But we still pass in the specific oldPart so that typeclass search for split_sepclause
+     can determine its length, either from a suchThat, or by computing it *)
+  Definition split_sepclause(oldAll oldPart: mem -> Prop)(stmt: Prop) := stmt.
+
+  Local Set Warnings "-notation-overridden".
+  Local Infix "++" := SeparationLogic.app. Local Infix "++" := app : list_scope.
+  Let nth n xs := SeparationLogic.hd (emp(map:=mem) True) (SeparationLogic.skipn n xs).
+  Let remove_nth n (xs : list (mem -> Prop)) :=
+    (SeparationLogic.firstn n xs ++ SeparationLogic.tl (SeparationLogic.skipn n xs)).
+
+  Lemma rewrite_ith_in_lhs_of_impl1: forall i Ps Pi Qs R,
+      nth i Ps = Pi ->
+      iff1 (seps Qs) Pi /\ (* <-- used right-to-left *)
+      impl1 (seps (remove_nth i Ps ++ Qs)) R ->
+      impl1 (seps Ps) R.
+  Proof.
+    intros. destruct H0. subst Pi.
+    unfold nth, remove_nth in *.
+    rewrite <-(seps_nth_to_head i Ps).
+    rewrite <- H0.
+    rewrite 2seps_app in H1. rewrite seps_app.
+    etransitivity. 2: eassumption.
+    ecancel.
+  Qed.
+
+  (* Transforms the goal so that goal modifications that are made while proving Rs
+     are still visible when proving the continuation Cont of the program *)
+  Lemma put_and_r_into_emp_seps: forall (Cont: Prop) (Rs: list (mem -> Prop)) (m: mem),
+      seps (SeparationLogic.app Rs [emp Cont]) m ->
+      seps Rs m /\ Cont.
+  Proof.
+    intros. change SeparationLogic.app with (@List.app (mem -> Prop)) in H.
+    apply seps_app in H. eapply sep_emp_r in H. assumption.
+  Qed.
+End SepLog.
+
+(* Hints for `(split_sepclause ?oldAll ?oldPart ?stmt)` goals *)
+Create HintDb split_sepclause_goal.
+
+(* Hints to solve the sideconditions of the `stmt` above, when using the iff1
+   right-to-left, ie in the split direction *)
+Create HintDb split_sepclause_sidecond.
+
+(* Hints to solve the sideconditions of the `stmt` above, when using the iff1
+   left-to-right, ie in the merge direction *)
+Create HintDb merge_sepclause_sidecond.
+
+#[global] Hint Opaque split_sepclause : split_sepclause_goal.
+
+Ltac split_ith_left_to_cancel_with_fst_right i :=
+  lazymatch goal with
+  | |- Lift1Prop.impl1 (seps ?L) (seps (?RHead :: ?RRest)) =>
+    eapply (rewrite_ith_in_lhs_of_impl1 i L);
+    cbn [hd app firstn tl skipn];
+    [ reflexivity | ];
+    (* Current goal is a conjunction of two subgoals:
+       - iff1 for right-to-left-rewrite that we'll derive from a split_sepclause instance
+       - new impl1 to be proven after this cancellation step *)
+    let Li := lazymatch goal with |- iff1 _ ?Li /\ impl1 _ _ => Li end in
+    let Sp := fresh "Sp" in
+    eassert (split_sepclause Li RHead _) as Sp;
+    [ (* can be left unsolved for debugging *)
+      try typeclasses eauto with split_sepclause_goal
+      (* typeclasses eauto instead of eauto because eauto unfolds split_sepclause
+         and then just does `exact H` for the last Prop in the context, and it
+         seems that `Hint Opaque` and `Hint Constants Opaque` don't fix that
+         (and `Opaque split_sepclause` would fix it, but also affects the conversion
+         algorithm) *)
+    | split;
+    [ lazymatch type of Sp with
+      | split_sepclause _ _ ?stmt =>
+          tryif is_evar stmt then
+            idtac (* debugging and typeclasses eauto above failed *)
+          else (
+            cbv [split_sepclause] in Sp;
+            eapply Sp;
+            (* sideconditions of Sp can be left unsolved for debugging *)
+            eauto with split_sepclause_sidecond
+          )
+      end
+    | (* this goal is the remaining impl1 after cancellation, and it's the only
+         goal supposed to remain open unless debugging *) ] ]
+  end.
+
+(* Poses split_sepclause lemmas as hypotheses in the context, forming a stack of
+   rewrite steps that have been performed, which can later be undone by
+   pop_split_sepclause_stack *)
+Ltac impl_ecancel_step_with_splitting :=
+  lazymatch goal with
+  | |- Lift1Prop.impl1 (seps ?L) _ =>
+    let iLi := index_and_element_of L in (* <-- multi-success! *)
+    let i := lazymatch iLi with (?i, _) => i end in
+    split_ith_left_to_cancel_with_fst_right i; []
+  end.
+
+Ltac use_sep_asm :=
+  match goal with
+  | H: seps _ ?m |- seps _ ?m =>
+    refine (Morphisms.subrelation_refl Lift1Prop.impl1 _ _ _ m H)
+  end.
+
+Ltac impl_ecancel :=
+  cancel_seps;
+  repeat (repeat (once ecancel_step_by_implication); try impl_ecancel_step_with_splitting).
+
+Ltac finish_impl_ecancel :=
+  match goal with
+  | |- impl1 ?R (seps [?E; emp ?P]) => is_evar E; refine (impl1_done R P _)
+  | |- impl1 ?x (seps [?E]) => is_evar E; change (impl1 x E); exact impl1_refl
+  | |- impl1 ?x ?y => first [ is_evar x | is_evar y | constr_eq x y ]; exact impl1_refl
+  | |- _ => pose_err Error:("impl_ecancel should cancel all clauses of this goal (except maybe one remaining emp)")
+  end.
+
+Ltac impl_ecancel_assumption :=
+  use_sep_asm;
+  impl_ecancel;
+  try finish_impl_ecancel.
+
+Ltac clear_split_sepclause_stack :=
+  repeat match goal with
+         | H: split_sepclause _ _ _ |- _ => clear H
+         end.
+
+Ltac pop_split_sepclause_stack :=
+  let H := lazymatch goal with H: seps _ ?m |- _ => H end in
+  let Sp := lazymatch goal with Sp: split_sepclause _ _ _ |- _ => Sp end in
+  ((cbv [split_sepclause] in Sp;
+    cbn [seps] in Sp, H;
+    seprewrite_in_by Sp H ltac:(eauto with merge_sepclause_sidecond)
+   ) || let T := type of Sp in idtac "Note: Failed to merge sep clauses using" T);
+  clear Sp.
+
+Ltac intro_new_mem :=
+  lazymatch goal with
+  | |- forall (m: @map.rep _ _ _), _ =>
+      let mNew := fresh m in
+      intro mNew; intros;
+      repeat pop_split_sepclause_stack
+  end.
+
+Ltac put_cont_into_emp_seps :=
+  lazymatch goal with
+  | |- seps ?Pre ?mOld /\ (forall mNew, _) =>
+      apply put_and_r_into_emp_seps; cbn [SeparationLogic.app]
+  | |- _ => fail 10000 "Expected a goal of the form" "(seps ?Pre ?mOld /\ (forall mNew, _))"
+  end.
+
+Ltac after_sep_call :=
+  put_cont_into_emp_seps;
+  use_sep_asm;
+  impl_ecancel;
+  match goal with
+  | _: tactic_error _ |- _ => idtac
+  | |- _ => finish_impl_ecancel;
+            match goal with
+            | _: tactic_error _ |- _ => idtac
+            | |- _ => intro_new_mem
+            end
+  end.
