bedrock2/src/bedrock2/TacticError.v
@@ -1,0 +1,48 @@
+(* Almost everyone importing this file will need strings in their error messages *)
+Require Import Coq.Strings.String. Open Scope string_scope.
+
+(* TODO The definition of dlist could/should be shared with compiler.util.Result *)
+Inductive dlist: Type :=
+| dnil
+| dcons{T: Type}(head: T)(tail: dlist).
+
+Declare Custom Entry ne_space_sep_dlist.
+Notation "x" := (dcons x dnil)
+  (in custom ne_space_sep_dlist at level 0, x constr at level 0).
+Notation "h t" := (dcons h t)
+  (in custom ne_space_sep_dlist at level 0,
+   h constr at level 0, t custom ne_space_sep_dlist at level 0).
+
+Inductive tactic_error(msg: dlist): Prop := mk_tactic_error.
+
+Declare Scope tactic_error_scope.
+Open Scope tactic_error_scope.
+
+(* Don't do this because even though it's only printing, it will conflict with
+   other "x" notations that use a different custom entry or constr for x
+Notation "x" := (tactic_error x)
+  (at level 0, x custom ne_space_sep_dlist at level 0, only printing)
+: tactic_error_scope. *)
+
+Notation "x !" := (tactic_error x)
+  (at level 0, x custom ne_space_sep_dlist at level 0, format "'[' x  ! ']'", only printing)
+: tactic_error_scope.
+
+Notation "'Error:(' msg )" := (mk_tactic_error msg)
+  (at level 0, msg custom ne_space_sep_dlist at level 0, format "'Error:(' msg )")
+  : tactic_error_scope.
+
+Ltac pose_err e := let n := fresh "Error" in pose proof e as n.
+
+Goal False.
+  pose_err Error:("Here's a very long error message that will take more than one line to display and I wonder how it will be rendered").
+  pose_err Error:("Here's a very long" (cons "really long" (cons "error message that" (cons "will take mooooooooooooooooooore than one line" nil))) "to display and I wonder how it will be rendered").
+  pose_err Error:(4 "is not a" bool).
+  pose_err Error:("just one string").
+Abort.
+
+Ltac assert_no_error :=
+  lazymatch goal with
+  | _: tactic_error _ |- _ => fail "You need to fix the error before continuing"
+  | |- _ => idtac
+  end.
