bedrock2/src/bedrock2/TransferSepsOrder.v
@@ -1,0 +1,183 @@
+(* Applying the order of sep clauses from an old hypothesis onto a new hypothesis: *)
+
+Require Export Coq.ZArith.ZArith. Open Scope Z_scope.
+Require Import coqutil.Z.Lia.
+Require Export coqutil.Byte.
+Require Import coqutil.Datatypes.HList.
+Require Import coqutil.Datatypes.PropSet.
+Require Export coqutil.Datatypes.Inhabited.
+Require Import coqutil.Tactics.rewr coqutil.Tactics.rdelta.
+Require Import Coq.Program.Tactics.
+Require Export coqutil.Tactics.Tactics.
+Require Export coqutil.Tactics.autoforward.
+Require Export coqutil.Map.Interface coqutil.Map.Properties coqutil.Map.OfListWord.
+Require Export coqutil.Word.Interface coqutil.Word.Properties.
+Require Import coqutil.Sorting.OrderToPermutation.
+Require Export coqutil.Tactics.fwd.
+Require Import coqutil.Tactics.ltac_list_ops.
+Require Export bedrock2.Lift1Prop.
+Require Export bedrock2.Map.Separation bedrock2.Map.SeparationLogic.
+Require Import bedrock2.Array.
+Require Export bedrock2.ZnWords.
+Require Import bedrock2.ptsto_bytes bedrock2.Scalars.
+Require Export bedrock2.SepAddrLast.
+Export List.ListNotations. Open Scope list_scope.
+
+Section TransferSepsOrder.
+  Context {width : Z} {word : Word.Interface.word width} {word_ok: word.ok word}
+          {mem : map.map word byte} {mem_ok: map.ok mem}.
+
+  Lemma reorder_is_iff1: forall (order: list nat) (l: list (mem -> Prop)),
+      List.length order = List.length l ->
+      iff1 (seps l) (seps (reorder order l)).
+  Proof.
+    intros. rewrite <-2seps'_iff1_seps. rewrite seps'_fold_right.
+    rewrite reorder_comm_fold_right.
+    - reflexivity.
+    - intros. eapply iff1ToEq. cancel.
+    - assumption.
+  Qed.
+End TransferSepsOrder.
+
+Lemma iff1_refl{A: Type}(P: A -> Prop): iff1 P P. Proof. reflexivity. Qed.
+Lemma iff1_sym{A: Type}{P Q: A -> Prop}: iff1 P Q -> iff1 Q P.
+Proof. intros. symmetry. assumption. Qed.
+
+Ltac iff1_syntactic_reflexivity :=
+  lazymatch goal with
+  | |- iff1 ?x ?y => first [is_evar x | is_evar y | constr_eq x y]
+  end;
+  exact (iff1_refl _).
+
+Ltac impl1_syntactic_reflexivity :=
+  lazymatch goal with
+  | |- impl1 ?x ?y => first [is_evar x | is_evar y | constr_eq x y]
+  end;
+  exact impl1_refl.
+
+Ltac clause_index clause clauses start_index default_index :=
+  lazymatch clauses with
+  | cons (at_addr ?a _) ?tail =>
+    lazymatch clause with
+    | at_addr a _ => constr:(start_index)
+    | _ => clause_index clause tail (S start_index) default_index
+    end
+  | cons clause _ => constr:(start_index)
+  | cons _ ?tail => clause_index clause tail (S start_index) default_index
+  | nil => constr:(default_index)
+  end.
+
+Ltac get_order_rec old_clauses new_clauses default_index :=
+  lazymatch new_clauses with
+  | nil => constr:(@nil nat)
+  | cons ?clause ?tail =>
+    let priority := clause_index clause old_clauses 0%nat default_index in
+    let rest := get_order_rec old_clauses tail priority in
+    constr:(priority :: rest)
+  end.
+
+Ltac get_order old_clauses new_clauses :=
+  (* if the first clause is not found in old_clauses, we put it at the end;
+     if a non-first clause is not found, we put it after the clause that's
+     to the left of it in new_clauses, so we give it the same priority value,
+     so the returned order might have duplicate priority values, and we rely
+     on mergesort being stable to keep the order between clauses of the same priority *)
+  let n := list_length old_clauses in
+  get_order_rec old_clauses new_clauses n.
+
+Ltac is_fresh x := assert_succeeds (pose proof tt as x).
+
+Ltac make_fresh x :=
+  tryif is_fresh x then idtac else let x' := fresh x "_0" in rename x into x'.
+
+(* Given `H: seplogformula m`, first cbns away all occurrences of `seps` in H,
+   and then flattens the formula into a list of sep clauses, resulting in an
+   `H: seps [...] m` *)
+Ltac flatten_seps_in H :=
+  lazymatch type of H with
+  | ?nested ?m =>
+    let tmem := type of m in
+    let E := fresh "E" in
+    eassert (@iff1 tmem nested _) as E;
+    [ (* from `nested` to `Tree.to_sep tree` *)
+      let stars := eval cbn[seps] in nested in
+      let tree := reify stars in
+      transitivity (Tree.to_sep tree); [
+        cbn [seps Tree.to_sep Tree.interp]; iff1_syntactic_reflexivity
+      |];
+      (* from `Tree.to_sep tree` to `seps (Tree.flatten tree)` *)
+      transitivity (seps (Tree.flatten tree)); [
+        exact (iff1_sym (Tree.flatten_iff1_to_sep tree))
+      |];
+      (* from `seps (Tree.flatten tree)` to `seps clauses` *)
+      cbn [SeparationLogic.Tree.flatten SeparationLogic.Tree.interp SeparationLogic.app];
+      iff1_syntactic_reflexivity
+    | let HNew := fresh in pose proof (proj1 (E m) H) as HNew;
+      move HNew before H;
+      clear E H;
+      rename HNew into H ]
+  end.
+
+(* Given an old and a new sep hyp, transfers the order of the sepclauses from the old one
+   to the new one *)
+Ltac transfer_sep_order_from_to HOld HNew :=
+  lazymatch type of HOld with
+  | seps ?old_clauses ?mOld =>
+    lazymatch type of HNew with
+    | seps ?new_clauses ?mNew =>
+      let tmem := type of mNew in
+      let E := fresh "E" in
+      eassert (@iff1 tmem (seps new_clauses) _) as E;
+      [ (* from `seps new_clauses` to `seps (reorder order new_clauses)` *)
+        let order := get_order old_clauses new_clauses in
+        etransitivity; [
+          eapply (reorder_is_iff1 order new_clauses); reflexivity
+        |];
+        (* from `seps (reorder order new_clauses)` to cbv'd version of it *)
+        cbv [reorder];
+        let r := eval vm_compute in (order_to_permutation order) in
+            change (order_to_permutation order) with r;
+        cbv [apply_permutation apply_permutation_with_default my_list_map my_list_nth];
+        reflexivity
+      | let HNewNew := fresh in pose proof (proj1 (E mNew) HNew) as HNewNew;
+        clear E HOld HNew;
+        rename HNewNew into HOld;
+        try clear mOld;
+        (* won't work if mNew or mOld is not a variable *)
+        try (make_fresh mOld; rename mNew into mOld) ]
+    end
+  end.
+
+Ltac transfer_sep_order :=
+  let mNew := lazymatch goal with mNew: @map.rep (@word.rep _ _) _ _ |- _ => mNew end in
+  lazymatch goal with
+  | HOld: seps _ ?mOld, HNew: _ mNew |- _ =>
+      flatten_seps_in HNew;
+      transfer_sep_order_from_to HOld HNew
+  end.
+
+Section TestTransferSepsOrder.
+  Context {width : Z} {word : Word.Interface.word width} {word_ok: word.ok word}
+          {mem : map.map word byte} {mem_ok: map.ok mem}.
+
+  Lemma reordering_test: forall addr1 addr2 addr3 addr4 v1_old v1_new v2 v3 v4 R (m m': mem),
+    seps [addr1 |-> scalar v1_old; addr2 |-> scalar v2; addr3 |-> scalar v3; R] m ->
+    (* value at addr1 was updated, addr2 was consumed, addr4 was added, and order changed: *)
+    seps [R; seps [addr3 |-> scalar v3; addr4 |-> scalar v4]; addr1 |-> scalar v1_new] m' ->
+    (* desired order:
+    seps [addr1 |-> scalar v1_new; addr3 |-> scalar v3; addr4 |-> scalar v4; R] m1 *)
+    True ->
+    True.
+  Proof.
+    intros *. intros M M2 ExtraHyp.
+    (*            0                        1                    2                    3
+       M  : seps [addr1 |-> scalar v1_old; addr2 |-> scalar v2; addr3 |-> scalar v3; R] m0
+       M2 : seps [R; addr3 |-> scalar v3; addr4 |-> scalar v4; addr1 |-> scalar v1_new] m1
+       order :=  [3; 2;                   2;                   0                      ] *)
+    flatten_seps_in M2.
+    transfer_sep_order_from_to M M2.
+    lazymatch type of M with
+    | seps [addr1 |-> scalar v1_new; addr3 |-> scalar v3; addr4 |-> scalar v4; R] m => idtac
+    end.
+  Abort.
+End TestTransferSepsOrder.
