bedrock2/src/bedrock2Examples/LiveVerif/LiveVerif.v
@@ -1,17 +1,26 @@
+Require Import Coq.ZArith.ZArith. Local Open Scope Z_scope.
 Require Import coqutil.Z.Lia.
 Require Import coqutil.Byte coqutil.Datatypes.HList.
 Require Import coqutil.Datatypes.PropSet.
+Require Import coqutil.Datatypes.Inhabited.
 Require Import coqutil.Tactics.letexists coqutil.Tactics.Tactics coqutil.Tactics.rewr coqutil.Tactics.rdelta.
 Require Import coqutil.Map.Interface coqutil.Map.Properties.
+Require coqutil.Map.SortedListString. (* for function env, other maps are kept abstract *)
 Require Import coqutil.Word.Interface coqutil.Word.Properties.
+Require Import coqutil.Tactics.fwd.
 Require Import bedrock2.Syntax bedrock2.Semantics.
 Require Import bedrock2.Lift1Prop.
 Require Import bedrock2.Map.Separation bedrock2.Map.SeparationLogic bedrock2.Array.
 Require Import bedrock2.ZnWords.
+Require Import bedrock2.groundcbv.
 Require Import bedrock2.ptsto_bytes bedrock2.Scalars.
 Require Import bedrock2.WeakestPrecondition bedrock2.ProgramLogic bedrock2.Loops.
 Require Import coqutil.Word.Bitwidth32.
 Require coqutil.Datatypes.String coqutil.Map.SortedList coqutil.Map.SortedListString.
+Require Import bedrock2Examples.LiveVerif.string_to_ident.
+Require Import bedrock2Examples.LiveVerif.ident_to_string.
+Require Import bedrock2.SepBulletPoints.
+Require Import bedrock2.SepAutoArray bedrock2.SepAuto.
 
 Infix "^+" := word.add  (at level 50, left associativity).
 Infix "^-" := word.sub  (at level 50, left associativity).
